ulib/FStar.Preorder.fst
@@ -6,6 +6,10 @@ type relation (a:Type) = a -> a -> Type0
 
 type predicate (a:Type) = a -> Type0
 
+let reflexive_rel (#a:Type) (rel:relation a) = forall (x:a). rel x x
+let transitive_rel (#a:Type) (rel:relation a) =
+  forall (x y z:a). rel x y /\ rel y z ==> rel x z
+
 let preorder_rel (#a:Type) (rel:relation a) =
   (forall (x:a). rel x x) /\ (forall (x:a) (y:a) (z:a). (rel x y /\ rel y z) ==> rel x z)
 
